made bloomfilters fintype

Structures/BloomFilter.v
@@ -21,16 +21,50 @@ Require Import Parameters Hash Comp Notationv1 BitVector.
    k - number of hashes
    n - maximum number of hashes supported
  *)
-Record BloomFilter k n := {
+Record BloomFilter k n := mkBloomFilter {
        bloomfilter_hashes: k.-tuple (HashState n);
        bloomfilter_state: BitVector
 }.
 
+Definition BloomFilter_prod k n (bf: BloomFilter k n) := (bloomfilter_hashes bf, bloomfilter_state bf).
+Definition prod_BloomFilter k n pair := let: (hashes, state) := pair in @mkBloomFilter k n hashes state.
+
+Lemma bloomfilter_cancel k n : cancel (@BloomFilter_prod k n) (@prod_BloomFilter k n).
+Proof.
+  by case.
+Qed.
+
+
+Definition bloomfilter_eqMixin k n :=
+  CanEqMixin (@bloomfilter_cancel k n).
+Canonical bloomfilter_eqType k n :=
+  Eval hnf in EqType (@BloomFilter k n) (bloomfilter_eqMixin k n).
+
+Definition bloomfilter_choiceMixin k n:=
+  CanChoiceMixin (@bloomfilter_cancel k n).
+Canonical bloomfilter_choiceType k n :=
+  Eval hnf in ChoiceType (@BloomFilter k n ) (bloomfilter_choiceMixin k n).
+
+Definition bloomfilter_countMixin k n :=
+  CanCountMixin (@bloomfilter_cancel k n).
+Canonical bloomfilter_countType k n :=
+  Eval hnf in CountType (@BloomFilter k n) (bloomfilter_countMixin k n).
+
+Definition bloomfilter_finMixin k n :=
+  CanFinMixin (@bloomfilter_cancel k n).
+Canonical bloomfilter_finType k n :=
+Eval hnf in FinType (@BloomFilter k n) (bloomfilter_finMixin k n).
 
 (* The first approximation: a number of axioms *)
 
-Definition bloomfilter_add k n (value: B) (bf: BloomFilter k n) : BloomFilter k n.
+Definition bloomfilter_add k n (value: B) (bf: BloomFilter k n) : Comp [finType of (BloomFilter k n)].
   Admitted.
+
+
+Fixpoint bloomfilter_add_internal k n (value: B) (bf: BloomFilter k n) : BloomFilter k n.
+Proof.
+  move: bf => [[xs H_xs] bvec].
+
 
 Definition bloomfilter_query k n (value: B) (bf: BloomFilter k n) : bool.
   Admitted.
